Checker for bitwise operations and equality

src/bva/Bva_checker.v
@@ -15,9 +15,8 @@
 (** A small checker for bit-vectors bit-blasting *)
 
 Require Import Int63 PArray.
-Require Import Bool List BoolEq NZParity.
-
 Require Import Misc State SMT_terms.
+Require Import Bool List BoolEq NZParity.
 
 
 Import Form.
@@ -33,29 +32,100 @@ Section Checker.
 
   Import Atom.
 
-
   Variable t_form : PArray.array form.
   Variable t_atom : PArray.array atom.
+  Variable s : S.t.
 
   Local Notation get_form := (PArray.get t_form) (only parsing).
   Local Notation get_atom := (PArray.get t_atom) (only parsing).
 
-  (* Ex of an LFSC rule: (x = y) ↔ (x₀ ↔ y₀ ∧ ... ∧ xₙ ↔ yₙ) *)
 
-  Definition check_bv_eq l :=
-    match get_form l with
-    | Fiff l1 l2 =>
-      match get_form l1, get_form l2 with
-      | Fatom a, Fand ls =>
-        match get_atom a with
-        | Abop (BO_eq Typ.TBV) h1 h2 =>
-          (* TODO: add the check for the rhs *)
-          if Lit.is_pos l then l::nil else C._true
-        | _ => C._true
+  (* Bit-blasting a variable *)
+
+  (* Definition check_bbVar a := *)
+  (*   ??                          (* need to known the length *) *)
+
+
+  (* Bit-blasting bitwise operations: bbAnd, bbOr, ... *)
+
+  Fixpoint check_op (bs1 bs2 bsres : list _lit) get_op :=
+    match bs1, bs2, bsres with
+    | nil, nil, nil => true
+    | b1::bs1, b2::bs2, bres::bsres =>
+      if Lit.is_pos bres then
+        match get_op (get_form bres) with
+        | Some (a1, a2) => (a1 == b1) && (a2 == b2)
+        | _ => false
         end
-      | _, _ => C._true
-      end
-    | _ => C._true
+      else false
+    | _, _, _ => false
+    end.
+
+  Definition get_and f :=
+    match f with
+    | Fand args => if PArray.length args == 2 then Some (args.[0], args.[1]) else None
+    | _ => None
+    end.
+
+  Definition get_or f :=
+    match f with
+    | For args => if PArray.length args == 2 then Some (args.[0], args.[1]) else None
+    | _ => None
+    end.
+
+  Definition check_bbOp pos1 pos2 lres :=
+    match S.get s pos1, S.get s pos2 with
+    | l1::nil, l2::nil =>
+      if (Lit.is_pos l1) && (Lit.is_pos l2) && (Lit.is_pos lres) then
+        match get_form l1, get_form l2, get_form lres with
+        | FbbT a1 bs1, FbbT a2 bs2, FbbT a bsres =>
+          match get_atom a with
+          | Abop BO_BVand a1' a2' =>
+            if (a1 == a1') && (a2 == a2') && (check_op bs1 bs2 bsres get_and)
+            then lres::nil
+            else C._true
+          | Abop BO_BVor a1' a2' =>
+            if (a1 == a1') && (a2 == a2') && (check_op bs1 bs2 bsres get_or)
+            then lres::nil
+            else C._true
+          | _ => C._true
+          end
+        | _, _, _ => C._true
+        end
+      else C._true
+    | _, _ => C._true
+    end.
+
+
+  (* Bit-blasting equality *)
+
+  Definition get_iff f :=
+    match f with
+    | Fiff l1 l2 => Some (l1, l2)
+    | _ => None
+    end.
+
+  Definition check_bbEq pos1 pos2 lres :=
+    match S.get s pos1, S.get s pos2 with
+    | l1::nil, l2::nil =>
+      if (Lit.is_pos l1) && (Lit.is_pos l2) && (Lit.is_pos lres) then
+        match get_form l1, get_form l2, get_form lres with
+        | FbbT a1 bs1, FbbT a2 bs2, Fiff leq lbb =>
+          match get_form leq, get_form lbb with
+          | Fatom a, Fand bsres =>
+            match get_atom a with
+            | Abop (BO_eq TBV) a1' a2' =>
+              if (a1 == a1') && (a2 == a2') && (check_op bs1 bs2 (PArray.to_list bsres) get_iff)
+              then lres::nil
+              else C._true
+            | _ => C._true
+            end
+          | _, _ => C._true
+          end
+        | _, _, _ => C._true
+        end
+      else C._true
+    | _, _ => C._true
     end.
 
 
@@ -73,8 +143,11 @@ Section Checker.
     Local Notation interp_form_hatom :=
       (Atom.interp_form_hatom t_i t_func t_atom).
 
+    Local Notation interp_form_hatom_bv :=
+      (Atom.interp_form_hatom_bv t_i t_func t_atom).
+
     Local Notation rho :=
-      (Form.interp_state_var interp_form_hatom t_form).
+      (Form.interp_state_var interp_form_hatom interp_form_hatom_bv t_form).
 
     Local Notation t_interp := (t_interp t_i t_func t_atom).
 
@@ -89,17 +162,17 @@ Section Checker.
 
     Let def_t_form : default t_form = Form.Ftrue.
     Proof.
-      destruct (Form.check_form_correct interp_form_hatom _ ch_form) as [H _]; destruct H; auto.
+      destruct (Form.check_form_correct interp_form_hatom interp_form_hatom_bv _ ch_form) as [H _]; destruct H; auto.
     Qed.
 
     Let wf_t_form : Form.wf t_form.
     Proof.
-      destruct (Form.check_form_correct interp_form_hatom _ ch_form) as [H _]; destruct H; auto.
+      destruct (Form.check_form_correct interp_form_hatom interp_form_hatom_bv _ ch_form) as [H _]; destruct H; auto.
     Qed.
 
     Let wf_rho : Valuation.wf rho.
     Proof.
-      destruct (Form.check_form_correct interp_form_hatom _ ch_form); auto.
+      destruct (Form.check_form_correct interp_form_hatom interp_form_hatom_bv _ ch_form); auto.
     Qed.
 
     Lemma lit_interp_true : Lit.interp rho Lit._true = true.
@@ -109,9 +182,9 @@ Section Checker.
     Qed.
 
 
-    Let rho_interp : forall x : int, rho x = Form.interp interp_form_hatom t_form (t_form.[ x]).
+    Let rho_interp : forall x : int, rho x = Form.interp interp_form_hatom interp_form_hatom_bv t_form (t_form.[ x]).
     Proof.
-      destruct (check_form_correct interp_form_hatom _ ch_form) as ((H,H0), _).
+      destruct (check_form_correct interp_form_hatom interp_form_hatom_bv _ ch_form) as ((H,H0), _).
       intros x;apply wf_interp_form;trivial.
     Qed.
 
@@ -127,7 +200,10 @@ Section Checker.
     Qed.
 
 
-    Lemma valid_check_bv_eq : forall l, C.valid rho (check_bv_eq l).
+    Lemma valid_check_bbOp pos1 pos2 lres : C.valid rho (check_bbOp pos1 pos2 lres).
+    Admitted.
+
+    Lemma valid_check_bbEq pos1 pos2 lres : C.valid rho (check_bbEq pos1 pos2 lres).
     Admitted.
 
   End Proof.
